Complete proof of loop-equivalence given assumptions on δ

hol/datadepsScript.sml
@@ -114,6 +114,12 @@ val emptyG_edges = store_thm(
   simp[emptyG_def]);
 val _ = export_rewrites ["emptyG_edges"]
 
+val emptyG_nodes = store_thm(
+  "emptyG_nodes",
+  ``emptyG.nodes = ∅``,
+  simp[emptyG_def]);
+val _ = export_rewrites ["emptyG_nodes"]
+
 val wfG_empty = store_thm(
   "wfG_empty",
   ``wfG emptyG``,
@@ -282,6 +288,21 @@ val add_action_def = Define`
          edges := (λsrc tgt. G.edges src tgt ∨
                              src = a ∧ touches a tgt ∧ tgt ∈ G.nodes) |>
 `;
+
+val IN_add_action = store_thm(
+  "IN_add_action",
+  ``a1 ∈ add_action a2 G ⇔ a1 = a2 ∨ a1 ∈ G``,
+  simp[add_action_def] >> rw[EQ_IMP_THM] >> simp[]);
+val _ = export_rewrites ["IN_add_action"]
+
+val add_action_edges = store_thm(
+  "add_action_edges",
+  ``(add_action a G).edges a1 a2 ⇔
+    ¬(a ∈ G) ∧ a1 = a ∧ a2 ∈ G ∧ touches a1 a2 ∨ G.edges a1 a2``,
+  rw[add_action_def] >> metis_tac[]);
+val _ = export_rewrites ["add_action_edges"]
+
+
 
 val add_action_lemma = prove(
   ``(∀a1 a2. R' a1 a2 ⇒ R a1 a2 ∨ a1 = a ∧ a2 ≠ a) ∧ (∀b. ¬R a b ∧ ¬R b a) ⇒
@@ -514,31 +535,6 @@ val imap_imap_o = store_thm(
   simp[graph_equality, IN_imap, imap_edges] >> rpt strip_tac >>
   dsimp[]);
 
-val example_t =
-  ``FOR (0,N)
-      (eval (vsub (f : num mvector))
-            [(λi. i + 1); vsub (h : num mvector)]
-            (λi rds. EL 0 rds + EL 1 rds + 1))``;
-
-val computation =
-    EVAL ``let N = 5 in
-           let f = ((λi. EL i [4;3;2;1;0]), 5) in
-           let h = ((λi. EL i [0;1;1;2;3]), 5) in
-             ^example_t ((λi. EL i [0;0;0;0;0;0]), 6)``
-
-
-(* C original:
-int N = 5;
-int A[6] = {0};
-int f[5] = {4,3,2,1,0};
-int h[5] = {0,1,1,2,3};
-
-for (int i= 0; i < N; i++)
-  A[f[i]] = A[i+1] + A [h[i]];
-
-
-*)
-
 val ddepR_def = Define`
   ddepR wf rfs i0 i ⇔
     i0 < i ∧ (wf i0 = wf i ∨
@@ -603,19 +599,6 @@ val mkEAction_o = store_thm(
        REWRITE_RULE [SINGL_DEF] SINGL_APPLY_MAP, MAP_MAP_o,
        combinTheory.o_ABS_R]);
 
-val IN_add_action = store_thm(
-  "IN_add_action",
-  ``a1 ∈ add_action a2 G ⇔ a1 = a2 ∨ a1 ∈ G``,
-  simp[add_action_def] >> rw[EQ_IMP_THM] >> simp[]);
-val _ = export_rewrites ["IN_add_action"]
-
-val add_action_edges = store_thm(
-  "add_action_edges",
-  ``(add_action a G).edges a1 a2 ⇔
-    ¬(a ∈ G) ∧ a1 = a ∧ a2 ∈ G ∧ touches a1 a2 ∨ G.edges a1 a2``,
-  rw[add_action_def] >> metis_tac[]);
-val _ = export_rewrites ["add_action_edges"]
-
 val IN_FOLD_add_action = store_thm(
   "IN_FOLD_add_action",
   ``a ∈ FOLDR (add_action o f) emptyG l ⇔ ∃i. MEM i l ∧ a = f i``,
@@ -677,10 +660,7 @@ val FOLD_add_action_edges = store_thm(
                SIMP_RULE (srw_ss()) [Once arithmeticTheory.FORALL_NUM]) >>
             `k < j0` by metis_tac [DECIDE ``¬(x < y) ⇔ y ≤ x``] >>
             map_every qexists_tac [`k`, `j0`] >> simp[]) >>
-        disj1_tac >> reverse conj_tac
-        >- metis_tac[MEM_EL] >>
-        qx_gen_tac `a` >> Cases_on `MEM a l` >> simp[] >>
-        `a ≠ h` by metis_tac[] >> simp[mkEAction_def]) >>
+        metis_tac[MEM_EL]) >>
     disj2_tac >>
     `∃j0. j = SUC j0` by (Cases_on `j` >> fs[]) >> fs[] >>
     map_every qexists_tac [`i0`, `j0`] >> simp[] >>
@@ -696,8 +676,8 @@ val FOLDR_add_action_nodes = store_thm(
 
 val INJ_COMPOSE_IMAGE = store_thm(
   "INJ_COMPOSE_IMAGE",
-  ``INJ (f o g) s t ⇒ INJ f (IMAGE g s) t``,
-  dsimp[INJ_THM] >> metis_tac[]);
+  ``INJ (f o g) s t ==> INJ f (IMAGE g s) t``,
+  ASM_SIMP_TAC (srw_ss() ++ boolSimps.DNF_ss) [INJ_THM] THEN METIS_TAC[]);
 
 val add_action_nodes = store_thm(
   "add_action_nodes",
@@ -732,6 +712,7 @@ val imap_ID = store_thm(
   "imap_ID",
   ``imap (λa. a.iter) G = G``,
   dsimp[graph_equality, imap_edges, iter_noop]);
+val _ = export_rewrites ["imap_ID"]
 
 val imap_CONG = store_thm(
   "imap_CONG",
@@ -741,12 +722,14 @@ val imap_CONG = store_thm(
 
 val ALL_DISTINCT_MAP_INJ = store_thm(
   "ALL_DISTINCT_MAP_INJ",
-  ``(∀x y. MEM x l ∧ MEM y l ⇒ (f x = f y ⇔ x = y)) ⇒
-    (ALL_DISTINCT (MAP f l) ⇔ ALL_DISTINCT l)``,
-  Induct_on `l` >> dsimp[MEM_MAP] >> metis_tac[]);
-(*
-val same_graphs = prove(
-  ``(∀i0 i. ddepR wf rfs i0 i ==> δ i0 < δ i) ∧
+  ``(!x y. MEM x l ∧ MEM y l ==> ((f x = f y) <=> (x = y))) ⇒
+    (ALL_DISTINCT (MAP f l) <=> ALL_DISTINCT l)``,
+  Induct_on `l` THEN ASM_SIMP_TAC (srw_ss() ++ boolSimps.DNF_ss) [MEM_MAP] THEN
+  METIS_TAC[]);
+
+val same_graphs = store_thm(
+  "same_graphs",
+  ``(∀i0 i. ddepR wf rds i0 i ==> δ i0 < δ i) ∧
     BIJ δ (count N) (count N) ∧
     γ = LINV δ (count N) ⇒
     loop_to_graph (0,N) (wf o γ) (MAP (λf. f o γ) rds) (body o γ) =
@@ -756,7 +739,8 @@ val same_graphs = prove(
      by metis_tac[IN_COUNT, BIJ_DEF, LINV_DEF, BIJ_LINV_INV] >>
   `∀n. n < N ⇒ γ n < N ∧ δ n < N`
      by metis_tac[BIJ_DEF, INJ_THM, BIJ_LINV_BIJ, IN_COUNT] >>
-  `∀m n. m < N ∧ n < N ⇒ (δ m = δ n ⇔ m = n)` by metis_tac[] >>
+  `(∀m n. m < N ∧ n < N ⇒ (δ m = δ n ⇔ m = n)) ∧
+   (∀m n. m < N ∧ n < N ⇒ (γ m = γ n ⇔ m = n))` by metis_tac[] >>
   simp[loop_to_graph_FOLDR] >>
   `MAP (γ o δ) [0 ..< N] = [0 ..< N]`
     by simp[LIST_EQ_REWRITE, EL_MAP, EL_listRangeLHI] >>
@@ -795,28 +779,134 @@ val same_graphs = prove(
     [FOLD_add_action_edges_ALL_DISTINCT, EL_MAP, EL_listRangeLHI] >>
   map_every qx_gen_tac [`a1`, `a2`] >> eq_tac >| [
     disch_then (qx_choosel_then [`i`, `j`] strip_assume_tac) >>
-    map_every qexists_tac [`γ i`, `γ j`] >> asimp[]  ddepR_def
+    map_every qexists_tac [`γ i`, `γ j`] >> asimp[] >>
+    qpat_assum `∀i0 i. ddepR wf rsf i0 i ⇒ δ i0 < δ i`
+      (qspecl_then [`γ j`, `γ i`] mp_tac) >>
+    simp[ddepR_def] >>
+    qmatch_abbrev_tac `¬(γ j < γ i) ∨ P ⇒ γ i < γ j` >>
+    `¬P`
+      by (qpat_assum `touches XX YY` mp_tac >>
+          simp[touches_def, Abbr`mk'`, mkEAction_def, Abbr`P`,
+               REWRITE_RULE [SINGL_DEF] SINGL_APPLY_PERMUTE,
+               REWRITE_RULE [SINGL_DEF] SINGL_APPLY_MAP,
+               MAP_MAP_o, combinTheory.o_ABS_R] >>
+          strip_tac >> simp[]) >> simp[] >>
+    `i < N` by decide_tac >>
+    `γ i ≠ γ j` by simp[] >> decide_tac,
 
+    disch_then (qx_choosel_then [`i`, `j`] strip_assume_tac) >>
+    map_every qexists_tac [`δ i`, `δ j`]  >> simp[] >>
+    first_x_assum match_mp_tac >> simp[ddepR_def] >>
+    pop_assum mp_tac >>
+    simp[touches_def, Abbr`mk'`, mkEAction_def,
+         REWRITE_RULE [SINGL_DEF] SINGL_APPLY_PERMUTE,
+         REWRITE_RULE [SINGL_DEF] SINGL_APPLY_MAP,
+         MAP_MAP_o, combinTheory.o_ABS_R]
+  ]);
 
-*)
+val FOLDR_add_actionf_nodes = store_thm(
+  "FOLDR_add_actionf_nodes",
+  ``(FOLDR (add_action o f) G l).nodes = { f e | MEM e l } ∪ G.nodes``,
+  Induct_on `l` >> simp[EXTENSION] >> metis_tac[]);
 
+val field_def = Define`field R = { x | (∃y. R x y) ∨ (∃y. R y x) }`
 
+val RIMAGE_TC_IN_field = store_thm(
+  "RIMAGE_TC_IN_field",
+  ``∀x y. (RIMAGE f R)⁺ x y ⇒
+          ∃x0 y0. x = f x0 ∧ y = f y0 ∧ x0 ∈ field R ∧ y0 ∈ field R``,
+  Induct_on `(RIMAGE f R)⁺` >> simp[RIMAGE_DEF] >> rpt strip_tac
+  >- (simp[field_def] >> metis_tac[]) >>
+  metis_tac[]);
 
+val INJ_RIMAGE_TC = store_thm(
+  "INJ_RIMAGE_TC",
+  ``INJ f (field R) SS ⇒
+    ∀x y. x ∈ field R ∧ y ∈ field R ∧ (RIMAGE f R)⁺ (f x) (f y) ⇒ R⁺ x y``,
+  strip_tac >>
+  `∀x y. (RIMAGE f R)⁺ x y ⇒
+         ∀x0 y0. x = f x0 ∧ y = f y0 ∧ x0 ∈ field R ∧ y0 ∈ field R ⇒ R⁺ x0 y0`
+     suffices_by metis_tac[] >>
+  Induct_on `(RIMAGE f R)⁺` >> simp[RIMAGE_DEF] >>
+  rpt strip_tac
+  >- (`a ∈ field R ∧ b ∈ field R` by (simp[field_def] >> metis_tac[]) >>
+      metis_tac[INJ_DEF, relationTheory.TC_SUBSET]) >>
+  qmatch_assum_rename_tac `(RIMAGE f R)⁺ x a` [] >>
+  qmatch_assum_rename_tac `(RIMAGE f R)⁺ a y` [] >>
+  `∃a0. a0 ∈ field R ∧ f a0 = a` by metis_tac[RIMAGE_TC_IN_field] >>
+  metis_tac[relationTheory.TC_RULES]);
 
+val wfG_imap = store_thm(
+  "wfG_imap",
+  ``wfG G ∧ INJ f G.nodes Is ⇒ wfG (imap f G)``,
+  simp[wfG_def, imap_def, RIMAGE_DEF] >> strip_tac >>
+  qabbrev_tac `f' = (λa. a with iter := f a)` >>
+  `∀a. a with iter := f a = f' a` by simp[Abbr`f'`] >>
+  simp[] >>
+  `∀a1 a2. a1 ∈ G ∧ a2 ∈ G ⇒ (f' a1 = f' a2 ⇔ a1 = a2)`
+    by (fs[INJ_THM,Abbr`f'`] >> simp[theorem "action_component_equality"] >>
+        simp[EQ_IMP_THM]) >>
+  `∀a b. (touches (f' a) b ⇔ touches a b) ∧ (touches a (f' b) ⇔ touches a b)`
+    by simp[Abbr`f'`] >>
+  rpt strip_tac >> simp[]
+  >- metis_tac[]
+  >- metis_tac[]
+  >- (eq_tac >> rpt strip_tac
+      >- (rw[] >> fs[] >> metis_tac[]) >>
+      rw[] >> fs[] >>
+      qmatch_rename_tac `D1 ∨ D2 ∨ ¬G.edges b c` ["D1", "D2"] >>
+      Cases_on `G.edges b c` >> simp[] >>
+      qmatch_rename_tac `f' a1 ≠ f' a2 ∨ f' a3 ≠ f' a4` [] >>
+      `a1 ∈ G ∧ a2 ∈ G ∧ a3 ∈ G ∧ a4 ∈ G` by metis_tac[] >>
+      simp[] >> Cases_on `a1 = a2` >> simp[] >> strip_tac >>
+      rw[] >> metis_tac[]) >>
+  `field G.edges ⊆ G.nodes`
+    by (simp[field_def, SUBSET_DEF] >> metis_tac[]) >>
+  `INJ f' (field G.edges) (IMAGE f' (field G.edges))`
+    by (simp[INJ_DEF] >> map_every qx_gen_tac [`a`, `b`] >>
+        strip_tac >> `a ∈ G ∧ b ∈ G` by metis_tac[SUBSET_DEF] >>
+        simp[]) >>
+  `∃a10 a20. a1 = f' a10 ∧ a2 = f' a20 ∧
+             a10 ∈ field G.edges ∧ a20 ∈ field G.edges`
+    by (match_mp_tac RIMAGE_TC_IN_field >> simp[]) >>
+  `a10 ∈ G ∧ a20 ∈ G` by metis_tac[SUBSET_DEF] >>
+  metis_tac[INJ_RIMAGE_TC]);
 
-(*
 val correctness = store_thm(
   "correctness",
-  ``(∀i0 i. ddepR wf rfs i0 i ==> δ i0 < δ i) ∧
+  ``(∀i0 i. ddepR wf rds i0 i ==> δ i0 < δ i) ∧
     BIJ δ (count N) (count N) ∧
     γ = LINV δ (count N)
   ==>
-    FOR (0,N) (eval wf rfs body) =
+    FOR (0,N) (eval wf rds body) =
     FOR (0,N) (eval (wf o γ)
                     (MAP (λf. f o γ) rds)
-                    body)``
+                    (body o γ))``,
+  strip_tac >> pop_assum (assume_tac o SYM) >>
+  `∀n. n < N ⇒ γ (δ n) = n ∧ δ (γ n) = n`
+     by metis_tac[IN_COUNT, BIJ_DEF, LINV_DEF, BIJ_LINV_INV] >>
+  `∀n. n < N ⇒ γ n < N ∧ δ n < N`
+     by metis_tac[BIJ_DEF, INJ_THM, BIJ_LINV_BIJ, IN_COUNT] >>
+  `(∀m n. m < N ∧ n < N ⇒ (δ m = δ n ⇔ m = n)) ∧
+   (∀m n. m < N ∧ n < N ⇒ (γ m = γ n ⇔ m = n))` by metis_tac[] >>
+  ONCE_REWRITE_TAC [FUN_EQ_THM] >>
+  qx_gen_tac `A` >>
+  assume_tac
+    (Q.INST [`lo` |-> `0`, `hi` |-> `N`, `rfs` |-> `rds`]
+            loop_to_graph_correct) >>
+  assume_tac
+    (Q.INST [`lo` |-> `0`, `hi` |-> `N`,
+             `rfs` |-> `MAP (λf. f o (γ:num->num)) rds`,
+             `wf` |-> `wf o γ`, `body` |-> `body o γ`]
+            loop_to_graph_correct) >>
+  mp_tac same_graphs >> simp[] >>
+  disch_then SUBST_ALL_TAC >>
+  qabbrev_tac `G = loop_to_graph (0,N) wf rds body` >>
+  `INJ (λa. δ a.iter) G.nodes (count N)`
+    by (simp[Abbr`G`, loop_to_graph_FOLDR,
+             FOLDR_add_actionf_nodes] >>
+        dsimp[INJ_DEF, mkEAction_def]) >>
+  `wfG G` by metis_tac[wfG_loop_to_graph] >>
+  metis_tac[imap_irrelevance, wfG_imap, wfG_evaluate_deterministically]);
 
-
-
-*)
 val _ = export_theory();
